

Bifurcation Equations

Kuznetsov Cancer Model

$$\dot{x} = \lambda y + \frac{\rho xy}{\eta + y} - \mu xy - \delta x + \sigma,$$

$$\dot{y} = \alpha y(1 - \beta y)(y - \beta_0) - \mu_1 xy,$$

$$\begin{aligned} \text{In[*]} := \text{SN} = & -4 \beta \eta^2 \lambda^5 \mu \mu^5 + \alpha^5 (-1 + \beta \beta_0)^2 (\beta^2 \delta \eta + \mu + \beta (\delta + \eta \mu - \rho))^2 \\ & (\delta \eta + \beta \theta^2 \mu + \beta \theta (\delta + \eta \mu - \rho))^2 (\delta^2 + (-\eta \mu + \rho)^2 - 2 \delta (\eta \mu + \rho)) + \\ & \alpha \eta \lambda^4 \mu^4 (\eta \mu^2 + 2 \beta \mu (\eta (9 \delta - 4 \eta \mu - 5 \rho) + \beta \theta (4 \delta - 9 \eta \mu + 4 \rho)) + \\ & \beta^2 \eta (\delta^2 + \beta \theta^2 \mu^2 - 8 \eta^2 \mu^2 + 2 \delta (9 \beta \theta \mu + 4 \eta \mu - \rho) - 2 \theta \eta \mu \rho + \rho^2 - 2 \beta \theta \mu (4 \eta \mu + 5 \rho))) - \\ & 2 \alpha^2 \lambda^3 \mu^3 (\eta \mu^2 (\beta \theta (\delta - 2 \eta \mu + \rho) - \eta (-2 \delta + \eta \mu + \rho)) + \\ & \beta \mu (\beta \theta \eta (14 \delta^2 - 25 \delta \eta \mu + 13 \eta^2 \mu^2 - 4 \delta \rho - 10 \rho^2) + 2 \beta \theta^2 (\delta^2 - 7 \delta \eta \mu + 8 \eta^2 \mu^2 - \\ & 2 \delta \rho - 7 \eta \mu \rho + \rho^2) + \eta^2 (16 \delta^2 - 13 \delta \eta \mu + \eta^2 \mu^2 - 18 \delta \rho - 5 \eta \mu \rho + 4 \rho^2))) + \\ & \beta^3 \eta^2 (-\beta \theta^3 \mu^2 (-2 \delta + \eta \mu + \rho) + \beta \theta^2 \mu (16 \delta^2 - 13 \delta \eta \mu + \eta^2 \mu^2 - 18 \delta \rho - 5 \eta \mu \rho + 4 \rho^2) + \\ & \eta (\delta^3 + \delta^2 (\eta \mu - 4 \rho) + 2 (\eta \mu - \rho)^3 - \delta (4 \eta^2 \mu^2 + \eta \mu \rho - 5 \rho^2))) + \\ & \beta \theta (2 \delta^3 + \delta^2 (13 \eta \mu - 5 \rho) + (4 \eta \mu - \rho) (-\eta \mu + \rho)^2 + \delta (-18 \eta^2 \mu^2 - 31 \eta \mu \rho + 4 \rho^2))) + \\ & \beta^2 \eta (\beta \theta^3 \mu^2 (\delta - 2 \eta \mu + \rho) + \beta \theta^2 \mu (14 \delta^2 - 25 \delta \eta \mu + 13 \eta^2 \mu^2 - 4 \delta \rho - 10 \rho^2) + \\ & \beta \theta (\delta^3 + 18 \eta^3 \mu^3 + \delta^2 (25 \eta \mu - \rho) + 4 \eta^2 \mu^2 \rho - 23 \eta \mu \rho^2 + \rho^3 - \delta (46 \eta^2 \mu^2 + 30 \eta \mu \rho + \rho^2))) + \\ & \eta (2 \delta^3 + \delta^2 (13 \eta \mu - 5 \rho) + (4 \eta \mu - \rho) (-\eta \mu + \rho)^2 + \delta (-18 \eta^2 \mu^2 - 31 \eta \mu \rho + 4 \rho^2))) + \alpha^3 \lambda^2 \\ & \mu^2 (\mu^2 (\eta^2 (6 \delta^2 + (-\eta \mu + \rho)^2 - 6 \delta (\eta \mu + \rho)) + \beta \theta^2 (\delta^2 + 6 \eta^2 \mu^2 - 6 \eta \mu \rho + \rho^2 - 2 \delta (3 \eta \mu + \rho)) + \\ & 2 \beta \theta \eta (3 \delta^2 + 3 \eta^2 \mu^2 - \eta \mu \rho - 2 \rho^2 - \delta (5 \eta \mu + \rho))) - \\ & 2 \beta \mu (\beta \theta^3 \mu (5 \delta^2 + 14 \eta^2 \mu^2 - 18 \eta \mu \rho + 5 \rho^2 - 2 \delta (9 \eta \mu + 5 \rho)) + \\ & \beta \theta \eta (-18 \delta^3 + (\eta \mu - 8 \rho) (-\eta \mu + \rho)^2 + 4 \delta^2 (6 \eta \mu + 7 \rho) + \delta (-8 \eta^2 \mu^2 + 9 \eta \mu \rho - 2 \rho^2)) + \\ & \eta^2 (-14 \delta^3 - (\eta \mu - \rho)^3 + 3 \delta^2 (5 \eta \mu + 8 \rho) - \delta (\eta^2 \mu^2 - 12 \eta \mu \rho + 11 \rho^2)) - \beta \theta^2 (5 \delta^3 - \\ & 15 \eta^3 \mu^3 + 18 \eta^2 \mu^2 \rho + 2 \eta \mu \rho^2 - 5 \rho^3 - 15 \delta^2 (\eta \mu + \rho) + \delta (24 \eta^2 \mu^2 + 13 \eta \mu \rho + 15 \rho^2))) + \\ & \beta^4 \eta^2 (\beta \theta^4 \mu^2 (6 \delta^2 + (-\eta \mu + \rho)^2 - 6 \delta (\eta \mu + \rho)) + \delta^2 \eta^2 (\delta^2 + (-\eta \mu + \rho)^2 - 2 \delta (\eta \mu + \rho)) + \\ & 2 \beta \theta^3 \mu (14 \delta^3 + (\eta \mu - \rho)^3 - 3 \delta^2 (5 \eta \mu + 8 \rho) + \delta (\eta^2 \mu^2 - 12 \eta \mu \rho + 11 \rho^2)) + \\ & 2 \beta \theta \delta \eta (3 \delta^3 + \delta^2 (\eta \mu - 11 \rho) + 5 (\eta \mu - \rho)^3 + \delta (-9 \eta^2 \mu^2 - 4 \eta \mu \rho + 13 \rho^2)) + \\ & \beta \theta^2 (6 \delta^4 + 6 \delta^3 (5 \eta \mu - 3 \rho) + 2 \delta (9 \eta \mu - 4 \rho) (-\eta \mu + \rho)^2 + \\ & (-\eta \mu + \rho)^4 + \delta^2 (-54 \eta^2 \mu^2 - 72 \eta \mu \rho + 19 \rho^2))) - \\ & 2 \beta^3 \eta (\beta \theta^4 \mu^2 (-3 \delta^2 - 3 \eta^2 \mu^2 + \eta \mu \rho + 2 \rho^2 + \delta (5 \eta \mu + \rho)) + \delta \eta^2 (-3 \delta^3 - 5 (\eta \mu - \rho)^3 + \\ & \delta^2 (-\eta \mu + 11 \rho) + \delta (9 \eta^2 \mu^2 + 4 \eta \mu \rho - 13 \rho^2)) + \beta \theta \eta (-5 \delta^4 + 5 (-\eta \mu + \rho)^4 - \\ & 5 \delta (-\eta \mu + \rho)^2 (6 \eta \mu + \rho) + \delta^3 (-8 \eta \mu + 15 \rho) + \delta^2 (39 \eta^2 \mu^2 + 12 \eta \mu \rho - 10 \rho^2)) + \\ & \beta \theta^3 \mu (-18 \delta^3 + (\eta \mu - 8 \rho) (-\eta \mu + \rho)^2 + 4 \delta^2 (6 \eta \mu + 7 \rho) + \delta (-8 \eta^2 \mu^2 + 9 \eta \mu \rho - 2 \rho^2)) + \end{aligned}$$

$$\begin{aligned}
& \beta^2 \left(-3 \delta^4 + (9 \eta \mu - 2 \rho) (\eta \mu - \rho)^3 + \delta^3 (-24 \eta \mu + 7 \rho) + \right. \\
& \quad \left. \delta^2 (58 \eta^2 \mu^2 + 50 \eta \mu \rho - 3 \rho^2) - \delta (39 \eta^3 \mu^3 - 53 \eta^2 \mu^2 \rho + 11 \eta \mu \rho^2 + 3 \rho^3) \right) + \\
& \beta^2 \left(\beta^4 \mu^2 (\delta^2 + 6 \eta^2 \mu^2 - 6 \eta \mu \rho + \rho^2 - 2 \delta (3 \eta \mu + \rho)) + 2 \beta^3 \mu (5 \delta^3 - 15 \eta^3 \mu^3 + 18 \eta^2 \mu^2 \rho + 2 \eta \mu \right. \\
& \quad \left. \rho^2 - 5 \rho^3 - 15 \delta^2 (\eta \mu + \rho) + \delta (24 \eta^2 \mu^2 + 13 \eta \mu \rho + 15 \rho^2)) + \eta^2 (6 \delta^4 + 6 \delta^3 (5 \eta \mu - 3 \rho) + \right. \\
& \quad \left. 2 \delta (9 \eta \mu - 4 \rho) (-\eta \mu + \rho)^2 + (-\eta \mu + \rho)^4 + \delta^2 (-54 \eta^2 \mu^2 - 72 \eta \mu \rho + 19 \rho^2)) + \right. \\
& \quad \left. \beta^2 (\delta^4 + \delta^3 (30 \eta \mu - 4 \rho) - (-\eta \mu + \rho)^2 (54 \eta^2 \mu^2 + 28 \eta \mu \rho - \rho^2) + \right. \\
& \quad \left. \delta^2 (-99 \eta^2 \mu^2 - 90 \eta \mu \rho + 6 \rho^2) + 2 \delta (58 \eta^3 \mu^3 - 21 \eta^2 \mu^2 \rho + 45 \eta \mu \rho^2 - 2 \rho^3)) + \right. \\
& \quad \left. 2 \beta^3 \eta (3 \delta^4 + \delta^3 (24 \eta \mu - 7 \rho) - (9 \eta \mu - 2 \rho) (\eta \mu - \rho)^3 + \delta^2 (-58 \eta^2 \mu^2 - 50 \eta \mu \rho + 3 \rho^2) + \right. \\
& \quad \left. \delta (39 \eta^3 \mu^3 - 53 \eta^2 \mu^2 \rho + 11 \eta \mu \rho^2 + 3 \rho^3)) \right) - 2 \alpha^4 \lambda \mu 1 \\
& (\mu^2 (-\beta^3 \mu (\delta^2 - 3 \delta \eta \mu + 2 \eta^2 \mu^2 - 2 \delta \rho - 3 \eta \mu \rho + \rho^2) + \delta \eta^2 (2 \delta^2 + (-\eta \mu + \rho)^2 - 3 \delta (\eta \mu + \rho)) + \\
& \quad \beta^3 \eta (3 \delta^3 - (\eta \mu - \rho)^3 - \delta^2 (4 \eta \mu + 5 \rho) + \delta (2 \eta^2 \mu^2 - 3 \eta \mu \rho + \rho^2)) + \\
& \quad \beta^2 (\delta^3 - (-\eta \mu + \rho)^2 (3 \eta \mu + \rho) - \delta^2 (2 \eta \mu + 3 \rho) + \delta (4 \eta^2 \mu^2 + 3 \eta \mu \rho + 3 \rho^2))) + \\
& \beta^5 \beta^3 \delta \eta^2 (\beta^4 \mu^2 (2 \delta^2 + (-\eta \mu + \rho)^2 - 3 \delta (\eta \mu + \rho)) + \delta^2 \eta^2 (\delta^2 + (-\eta \mu + \rho)^2 - 2 \delta (\eta \mu + \rho)) + \\
& \quad \beta^3 \mu (6 \delta^3 + 2 (\eta \mu - \rho)^3 - 7 \delta^2 (\eta \mu + 2 \rho) - \delta (\eta^2 \mu^2 + 9 \eta \mu \rho - 10 \rho^2)) + \beta^2 (2 \delta^4 + 7 \delta^3 \\
& \quad (\eta \mu - \rho) + \delta (6 \eta \mu - 5 \rho) (-\eta \mu + \rho)^2 + (-\eta \mu + \rho)^4 + \delta^2 (-16 \eta^2 \mu^2 - 19 \eta \mu \rho + 9 \rho^2)) + \\
& \quad \beta^3 \delta \eta (3 \delta^3 + 4 (\eta \mu - \rho)^3 - \delta^2 (\eta \mu + 10 \rho) + \delta (-6 \eta^2 \mu^2 - 5 \eta \mu \rho + 11 \rho^2))) + \\
& \beta \mu (2 \beta^4 \mu^2 (2 \delta^2 - 5 \delta \eta \mu + 3 \eta^2 \mu^2 - 4 \delta \rho - 5 \eta \mu \rho + 2 \rho^2) - \beta^3 \eta (-10 \delta^4 - 4 \delta (2 \eta \mu - \rho) \\
& \quad (-\eta \mu + \rho)^2 + 2 (-\eta \mu + \rho)^4 + \delta^3 (9 \eta \mu + 28 \rho) + \delta^2 (7 \eta^2 \mu^2 + 15 \eta \mu \rho - 24 \rho^2)) + \\
& \quad \delta \eta^2 (6 \delta^3 + 2 (\eta \mu - \rho)^3 - 7 \delta^2 (\eta \mu + 2 \rho) - \delta (\eta^2 \mu^2 + 9 \eta \mu \rho - 10 \rho^2)) + \\
& \quad \beta^3 \mu (2 \delta^3 - 6 \delta^2 \rho + (7 \eta \mu - 2 \rho) (-\eta \mu + \rho)^2 + \delta (-9 \eta^2 \mu^2 - 11 \eta \mu \rho + 6 \rho^2)) + \\
& \quad \beta^2 (4 \delta^4 - 16 \delta^3 \rho - (\eta \mu - \rho)^3 (\eta \mu + 4 \rho) + \delta^2 (-10 \eta^2 \mu^2 - 11 \eta \mu \rho + 24 \rho^2) + \\
& \quad \delta (7 \eta^3 \mu^3 - 13 \eta^2 \mu^2 \rho + 22 \eta \mu \rho^2 - 16 \rho^3))) - \\
& \beta^4 \eta (-\delta^3 \eta^3 (\delta^2 + (-\eta \mu + \rho)^2 - 2 \delta (\eta \mu + \rho)) + \beta^4 \mu (-10 \delta^4 - 4 \delta (2 \eta \mu - \rho) (-\eta \mu + \rho)^2 + \\
& \quad 2 (-\eta \mu + \rho)^4 + \delta^3 (9 \eta \mu + 28 \rho) + \delta^2 (7 \eta^2 \mu^2 + 15 \eta \mu \rho - 24 \rho^2)) + \\
& \quad \beta^5 \mu^2 (-3 \delta^3 + (\eta \mu - \rho)^3 + \delta^2 (4 \eta \mu + 5 \rho) - \delta (2 \eta^2 \mu^2 - 3 \eta \mu \rho + \rho^2)) + \\
& \quad 2 \beta^3 \delta^2 \eta^2 (-\delta^3 + (\eta \mu - \rho)^3 + \delta^2 (4 \eta \mu + \rho) + \delta (-4 \eta^2 \mu^2 + 3 \eta \mu \rho + \rho^2)) + \beta^2 \delta \eta \\
& \quad (-4 \delta^4 + 10 \delta \rho (-\eta \mu + \rho)^2 - 2 (-\eta \mu + \rho)^4 + 7 \delta^3 (\eta \mu + 2 \rho) - \delta^2 (\eta^2 \mu^2 - 5 \eta \mu \rho + 18 \rho^2)) + \\
& \quad \beta^3 (-3 \delta^5 + (\eta \mu - \rho)^5 - \delta (\eta \mu - \rho)^3 (8 \eta \mu + \rho) + \delta^4 (-9 \eta \mu + 11 \rho) + \\
& \quad \delta^3 (18 \eta^2 \mu^2 + 33 \eta \mu \rho - 14 \rho^2) + \delta^2 (\eta^3 \mu^3 + 27 \eta^2 \mu^2 \rho - 34 \eta \mu \rho^2 + 6 \rho^3))) - \\
& \beta^2 (\beta^5 \mu^3 (\delta^2 - 3 \delta \eta \mu + 2 \eta^2 \mu^2 - 2 \delta \rho - 3 \eta \mu \rho + \rho^2) + \beta^4 \mu^2 \\
& \quad (-2 \delta^3 + 6 \delta^2 \rho - (7 \eta \mu - 2 \rho) (-\eta \mu + \rho)^2 + \delta (9 \eta^2 \mu^2 + 11 \eta \mu \rho - 6 \rho^2)) - \\
& \quad \delta \eta^2 (2 \delta^4 + 7 \delta^3 (\eta \mu - \rho) + \delta (6 \eta \mu - 5 \rho) (-\eta \mu + \rho)^2 + (-\eta \mu + \rho)^4 + \\
& \quad \delta^2 (-16 \eta^2 \mu^2 - 19 \eta \mu \rho + 9 \rho^2)) + 2 \beta^3 \mu (\delta^4 - (\eta \mu - \rho)^3 (8 \eta \mu + \rho) - \\
& \quad \delta^3 (3 \eta \mu + 4 \rho) + \delta^2 (\eta^2 \mu^2 + 11 \eta \mu \rho + 6 \rho^2) + \delta (9 \eta^3 \mu^3 + 8 \eta^2 \mu^2 \rho - 13 \eta \mu \rho^2 - 4 \rho^3)) + \\
& \quad \beta^2 (-\delta^5 + 5 \delta^4 \rho - (6 \eta \mu - \rho) (-\eta \mu + \rho)^4 - \delta (-\eta \mu + \rho)^2 (\eta^2 \mu^2 - 20 \eta \mu \rho + 5 \rho^2) - \\
& \quad 2 \delta^3 (\eta^2 \mu^2 - 5 \eta \mu \rho + 5 \rho^2) + 2 \delta^2 (5 \eta^3 \mu^3 + 9 \eta^2 \mu^2 \rho - 15 \eta \mu \rho^2 + 5 \rho^3)) + \\
& \quad \beta^3 \eta (-3 \delta^5 + (\eta \mu - \rho)^5 - \delta (\eta \mu - \rho)^3 (8 \eta \mu + \rho) + \delta^4 (-9 \eta \mu + 11 \rho) + \\
& \quad \delta^3 (18 \eta^2 \mu^2 + 33 \eta \mu \rho - 14 \rho^2) + \delta^2 (\eta^3 \mu^3 + 27 \eta^2 \mu^2 \rho - 34 \eta \mu \rho^2 + 6 \rho^3))) + \\
& \beta^3 (\beta^5 \mu^2 (\delta^3 - (-\eta \mu + \rho)^2 (3 \eta \mu + \rho) - \delta^2 (2 \eta \mu + 3 \rho) + \delta (4 \eta^2 \mu^2 + 3 \eta \mu \rho + 3 \rho^2)) + \\
& \quad \delta^2 \eta^3 (3 \delta^3 + 4 (\eta \mu - \rho)^3 - \delta^2 (\eta \mu + 10 \rho) + \delta (-6 \eta^2 \mu^2 - 5 \eta \mu \rho + 11 \rho^2)) + \beta^3 \delta \eta^2 \\
& \quad (4 \delta^4 - 10 \delta \rho (-\eta \mu + \rho)^2 + 2 (-\eta \mu + \rho)^4 - 7 \delta^3 (\eta \mu + 2 \rho) + \delta^2 (\eta^2 \mu^2 - 5 \eta \mu \rho + 18 \rho^2)) +
\end{aligned}$$

$$\begin{aligned}
& 2\beta\theta^2\eta\left(\delta^5+2(\eta\mu-\rho)^5-9\delta(\eta\mu-\rho)^3\rho-\delta^4(5\eta\mu+6\rho)+\right. \\
& \quad \left.\delta^3(5\eta^2\mu^2+3\eta\mu\rho+14\rho^2)+\delta^2(-3\eta^3\mu^3+19\eta\mu\rho^2-16\rho^3)\right)+ \\
& \beta\theta^3\left(\delta^5-5\delta^4\rho+(6\eta\mu-\rho)(-\eta\mu+\rho)^4+\delta(-\eta\mu+\rho)^2(\eta^2\mu^2-20\eta\mu\rho+5\rho^2)+\right. \\
& \quad \left.2\delta^3(\eta^2\mu^2-5\eta\mu\rho+5\rho^2)-2\delta^2(5\eta^3\mu^3+9\eta^2\mu^2\rho-15\eta\mu\rho^2+5\rho^3)\right)- \\
& \beta\theta^4\mu\left(-4\delta^4+16\delta^3\rho+(\eta\mu-\rho)^3(\eta\mu+4\rho)+\delta^2(10\eta^2\mu^2+11\eta\mu\rho-24\rho^2)+\right. \\
& \quad \left.\delta(-7\eta^3\mu^3+13\eta^2\mu^2\rho-22\eta\mu\rho^2+16\rho^3)\right)\Big);
\end{aligned}$$

$$\begin{aligned}
In[*]:= \text{Hopf} = & -\lambda^2\mu^3\mu_1^2+\alpha^6\beta\theta(-1+\beta\beta\theta)^2(\beta\theta+\eta)(1+\beta\eta) \\
& ((1+\beta(\beta\theta+2\eta))(2\beta\delta+\mu+\beta\beta\theta\mu)-2\beta(1+\beta\beta\theta)\rho)-2\alpha\beta\lambda^2\mu_1^2(-3\delta\mu+2\lambda\mu_1+3\mu\rho)- \\
& \alpha^5(\delta(\beta\theta+\eta)\mu-\beta\theta\mu\rho+\beta^5\beta\theta^2\delta\eta(\beta\theta+\eta)((\beta\theta+2\eta)(2\delta+\beta\theta\mu)-2\beta\theta\rho)+ \\
& \beta((\beta\theta+\eta)(2\delta^2+3\delta\eta\mu+4\beta\theta\lambda\mu_1)-2(2\beta\theta\delta+\delta\eta+\beta\theta\eta\mu)\rho+2\beta\theta\rho^2)+ \\
& 2\beta^2(-((\beta\theta+\eta)(\delta(\beta\theta^2\mu+\beta\theta(\delta+\eta\mu)-\eta(3\delta+\eta\mu))-2\beta\theta(2\beta\theta+3\eta)\lambda\mu_1))+ \\
& (\delta(2\beta\theta^2-2\beta\theta\eta-\eta^2)+\beta\theta^2(\beta\theta+\eta)\mu)\rho-\beta\theta^2\rho^2)+ \\
& 2\beta^3((\beta\theta+\eta)(\delta(-\delta(\beta\theta^2+5\beta\theta\eta-2\eta^2)-\beta\theta\eta(2\beta\theta+\eta)\mu)+2\beta\theta(\beta\theta^2+4\beta\theta\eta+2\eta^2)\lambda\mu_1)+ \\
& \beta\theta(6\beta\theta\delta\eta+\delta\eta^2+\beta\theta^2(2\delta+\eta\mu))\rho-\beta\theta^3\rho^2)+ \\
& \beta^4\beta\theta((\beta\theta+\eta)(\delta(-8\delta\eta^2+\beta\theta^3\mu+2\beta\theta\eta(\delta-\eta\mu)+2\beta\theta^2(\delta+\eta\mu))+4\beta\theta\eta(\beta\theta+2\eta)\lambda\mu_1)- \\
& \beta\theta(4\beta\theta\delta\eta-2\delta\eta^2+\beta\theta^3\mu+2\beta\theta^2(2\delta+\eta\mu))\rho+2\beta\theta^3\rho^2))- \\
& \alpha^3\lambda\mu_1(\mu(\delta-\rho)+\beta(2\delta^2+4(2\beta\theta+\eta)\lambda\mu_1+(7\beta\theta-2\eta)\mu\rho+2\rho^2-\delta(7\beta\theta\mu+6\eta\mu+4\rho))+ \\
& \beta^2(6\eta^2(-3\delta\mu+2\lambda\mu_1)+\beta\theta^2(-7\delta\mu+8\lambda\mu_1+7\mu\rho)- \\
& 4\beta\theta(\delta^2+6\delta\eta\mu-4\eta\lambda\mu_1-2\delta\rho-\eta\mu\rho+\rho^2))+ \\
& \beta^3(6\beta\theta\eta^2(-3\delta\mu+2\lambda\mu_1)+\beta\theta^3\mu(\delta-\rho)+4\eta^2(-3\delta\eta\mu+2\eta\lambda\mu_1+3\delta\rho)+ \\
& 2\beta\theta^2(\delta^2-3\delta\eta\mu+2\eta\lambda\mu_1-2\delta\rho-\eta\mu\rho+\rho^2)))- \\
& \alpha^2\lambda\mu_1(\mu(-\lambda\mu_1+\mu(\delta+2\beta\theta\mu+\eta\mu-\rho))+\beta(3\delta^2\mu+4\beta\theta\delta\mu^2+2\beta\theta^2\mu^3+4\beta\theta\eta\mu^3+ \\
& 3\eta^2\mu^3-6\delta\lambda\mu_1+2\beta\theta\lambda\mu\mu_1-2\mu(3\delta+2\beta\theta\mu+3\eta\mu)\rho+6\lambda\mu_1\rho+3\mu\rho^2)+ \\
& \beta^2(2\delta^3+\eta(\beta\theta+\eta)(\beta\theta+2\eta)\mu^3-\beta\theta^2\lambda\mu\mu_1+3\delta^2(\beta\theta\mu-2\rho)- \\
& (\beta\theta^2+6\beta\theta\eta+6\eta^2)\mu^2\rho+6(\beta\theta+2\eta)\lambda\mu_1\rho+3(\beta\theta+2\eta)\mu\rho^2- \\
& 2\rho^3+\delta(\beta\theta(\beta\theta\mu^2-6\lambda\mu_1)-6(\beta\theta+\eta)\mu\rho+6\rho^2)))- \\
& \alpha^4(\mu(\beta\theta^2\mu^2-2\beta\theta\lambda\mu_1+\eta(\delta\mu-\lambda\mu_1)+\beta\theta\mu(\delta+\eta\mu-\rho))+ \\
& \beta^4\eta((\beta\theta+\eta)(\beta\theta+2\eta)(\delta(\delta+\beta\theta\mu)(2\delta+\beta\theta\mu)-\beta\theta\lambda(6\delta+\beta\theta\mu)\mu_1)- \\
& \beta\theta(\delta(6\delta\eta+3\beta\theta^2\mu+4\beta\theta(\delta+\eta\mu))-2\beta\theta(\beta\theta+\eta)\lambda\mu_1)\rho+2\beta\theta^2\delta\rho^2)+\beta(2\beta\theta^3\mu^3+ \\
& \beta\theta^2\mu(2\lambda\mu_1+5\mu(\delta+\eta\mu-\rho))+\eta(3\delta^2\mu+\lambda\mu_1(-3\eta\mu+2\rho)+3\delta(\eta\mu^2-2\lambda\mu_1-\mu\rho))+ \\
& \beta\theta(3\delta^2\mu+3\eta^2\mu^3+\delta(8\eta\mu^2-8\lambda\mu_1-6\mu\rho)-2\eta\mu(\lambda\mu_1+3\mu\rho)+\rho(8\lambda\mu_1+3\mu\rho)))+ \\
& \beta^2(\beta\theta^4\mu^3+\beta\theta^3\mu(2\lambda\mu_1+5\mu(\delta+\eta\mu-\rho))+2\beta\theta^2 \\
& (3\delta^2\mu+3\eta^2\mu^3+\delta(9\eta\mu^2-4\lambda\mu_1-6\mu\rho)+3\eta\mu(\lambda\mu_1-2\mu\rho)+\rho(4\lambda\mu_1+3\mu\rho))+ \\
& \eta(2\delta^3+\delta^2(9\eta\mu-4\rho)+2\eta\lambda\mu_1(-\eta\mu+\rho)+2\delta(\eta^2\mu^2-9\eta\lambda\mu_1-2\eta\mu\rho+\rho^2))+ \\
& \beta\theta(2\delta^3+2\eta^3\mu^3+3\delta^2(5\eta\mu-2\rho)-2\rho^3+3\eta^2\mu(\lambda\mu_1-2\mu\rho)+ \\
& 2\eta\rho(5\lambda\mu_1+3\mu\rho)+3\delta(5\eta(\eta\mu^2-2\lambda\mu_1)-7\eta\mu\rho+2\rho^2)))+ \\
& \beta^3(\beta\theta^4\mu(-2\lambda\mu_1+\mu(\delta+\eta\mu-\rho))+6\delta\eta^2(\delta^2+\delta\eta\mu-2\eta\lambda\mu_1-\delta\rho)+ \\
& \beta\theta^3(3\delta^2\mu+3\eta^2\mu^3+\delta(8\eta\mu^2-8\lambda\mu_1-6\mu\rho)-2\eta\mu(\lambda\mu_1+3\mu\rho)+\rho(8\lambda\mu_1+3\mu\rho))+ \\
& \beta\theta^2(2\delta^3+2\eta^3\mu^3+3\delta^2(5\eta\mu-2\rho)-2\rho^3+3\eta^2\mu(\lambda\mu_1-2\mu\rho)+ \\
& 2\eta\rho(5\lambda\mu_1+3\mu\rho)+3\delta(5\eta(\eta\mu^2-2\lambda\mu_1)-7\eta\mu\rho+2\rho^2))+ \\
& 2\beta\theta\eta(4\delta^3+\delta^2(9\eta\mu-8\rho)+2\eta\lambda\mu_1(\eta\mu-\rho)+2\delta(2\eta^2\mu^2-9\eta\lambda\mu_1-4\eta\mu\rho+2\rho^2))));
\end{aligned}$$

$$\begin{aligned}
In[*]:= \text{BT} = & -3\eta\lambda^2\mu^3\mu_1^2\rho+\alpha^6(-1+\beta\beta\theta)^2\eta(\beta\theta+\eta) \\
& (1+\beta\eta)((1+\beta(\beta\theta+2\eta))^2\mu-4\beta^2\eta\rho)(\delta(\eta+\beta\beta\theta\eta)+\beta\theta(-\eta\mu+\rho))+
\end{aligned}$$

$$\begin{aligned}
& \alpha \lambda \mu^1 \left(\beta \theta \mu^2 \left(3 \beta \eta^3 \mu^3 + 3 \delta^2 (\mu + \beta \eta \mu) + 3 \mu \rho^2 - 6 \delta (1 + \beta \eta) \mu (\eta \mu + \rho) + 3 \eta^2 \mu^2 (\mu - 2 \beta \rho) + \right. \right. \\
& \quad \left. \left. \eta \rho (-6 \mu^2 + 2 \beta \lambda \mu^1 + 3 \beta \mu \rho) \right) + \eta \left(3 \beta \eta^3 \mu^5 + 3 \eta^2 \mu^4 (\mu - 3 \beta \rho) + 3 \delta^2 \mu^2 (\mu + \beta \eta \mu - \beta \rho) + \right. \right. \\
& \quad \left. \left. 3 \eta \mu^3 \rho (-2 \mu + 3 \beta \rho) + \rho (-4 \beta \lambda^2 \mu^1 + 2 \lambda \mu \mu^1 (\mu - 8 \beta \rho) + 3 \mu^2 \rho (\mu - \beta \rho)) - \right. \right. \\
& \quad \left. \left. 2 \delta (3 \eta \mu^4 + 3 \beta \eta^2 \mu^4 + \mu \rho (3 \mu^2 - 8 \beta \lambda \mu^1 - 3 \beta \mu \rho)) \right) \right) + \\
& \alpha^5 \eta (\beta \theta + \eta) (1 + \beta \eta) \left(-\mu (-2 \delta^2 + \eta \lambda \mu^1 + 2 \delta (\beta \theta \mu - \eta \mu + \rho)) + \right. \\
& \quad \left. 2 \beta (5 \delta^2 \eta \mu + \delta (\beta \theta^2 \mu^2 + 2 \beta \theta \mu (-\eta \mu + \rho) + 2 \eta (3 \eta \mu^2 - \lambda \mu^1 - 3 \mu \rho)) - \right. \\
& \quad \left. 2 (\eta^2 \lambda \mu \mu^1 + 2 \beta \theta^2 \mu^2 (\eta \mu - \rho) + \beta \theta (\eta \mu - \rho) (\eta \mu^2 - \lambda \mu^1 - \mu \rho)) \right) + \\
& \beta^4 (32 \delta^3 \eta^3 + 8 \beta \theta \delta \eta^2 (4 \delta^2 + 3 \delta \eta \mu - 2 \eta \lambda \mu^1 - 3 \delta \rho) + \beta \theta^4 \mu (2 \delta^2 + 2 \delta \eta \mu - \eta \lambda \mu^1 - 2 \delta \rho) + \\
& \quad 2 \beta \theta^3 \eta (5 \delta^2 \mu - 2 \eta \lambda \mu \mu^1 + \delta (6 \eta \mu^2 - 2 \lambda \mu^1 - 6 \mu \rho)) + \\
& \quad 4 \beta \theta^2 \eta (2 \delta^3 + 6 \delta^2 (\eta \mu - \rho) + \eta \lambda \mu^1 (-\eta \mu + \rho) + 4 \delta (\eta^2 \mu^2 - \eta \lambda \mu^1 - 2 \eta \mu \rho + \rho^2)) + \\
& \quad 2 \beta^2 (4 \delta^3 \eta + 4 \beta \theta^3 \mu^2 (-\eta \mu + \rho) + 2 \eta^2 \lambda \mu^1 (-\eta \mu + \rho) + \delta^2 (-2 \beta \theta^2 \mu + 12 \eta (\eta \mu - \rho) + \\
& \quad \beta \theta (7 \eta \mu + 4 \rho)) - 2 \beta \theta (2 \eta^3 \mu^3 - 2 \rho^3 + 2 \eta \rho (2 \lambda \mu^1 + 3 \mu \rho) - \eta^2 \mu (5 \lambda \mu^1 + 6 \mu \rho)) + \\
& \quad \beta \theta^2 (-12 \eta^2 \mu^3 - 4 \rho (\lambda \mu^1 + 3 \mu \rho) + \eta \mu (5 \lambda \mu^1 + 24 \mu \rho)) + \delta (\beta \theta^3 \mu^2 + 2 \beta \theta^2 \mu (\eta \mu + 7 \rho) + \\
& \quad 8 \eta (\eta^2 \mu^2 - \eta \lambda \mu^1 - 2 \eta \mu \rho + \rho^2) - 2 \beta \theta (3 \eta^2 \mu^2 + 3 \eta \lambda \mu^1 - 7 \eta \mu \rho + 4 \rho^2)) - 2 \beta^3 \\
& \quad (\beta \theta^4 \delta \mu^2 + 4 \delta \eta^2 (-4 \delta^2 - 3 \delta \eta \mu + 2 \eta \lambda \mu^1 + 3 \delta \rho) + 2 \beta \theta^3 (\eta \mu - \rho) (\delta \mu + \eta \mu^2 - \lambda \mu^1 - \mu \rho) + \\
& \quad 4 \beta \theta \eta (-2 \delta^3 + 3 \eta \lambda \mu^1 (-\eta \mu + \rho) - 2 \delta^2 (3 \eta \mu + \rho) + 4 \delta (\eta^2 \mu^2 + \eta \lambda \mu^1 - 2 \eta \mu \rho + \rho^2)) + \\
& \quad \beta \theta^2 (4 \eta^3 \mu^3 - 4 \rho^3 - \delta^2 (7 \eta \mu + 4 \rho) + 4 \eta \rho (2 \lambda \mu^1 + 3 \mu \rho) - \\
& \quad 2 \eta^2 \mu (5 \lambda \mu^1 + 6 \mu \rho) + 2 \delta (3 \eta^2 \mu^2 + 3 \eta \lambda \mu^1 - 7 \eta \mu \rho + 4 \rho^2)) + \\
& \alpha^2 (\mu (3 \beta \theta^2 \mu^3 (\delta^2 + (-\eta \mu + \rho)^2 - 2 \delta (\eta \mu + \rho)) + \eta (3 \delta^3 \mu^2 - 2 \delta^2 \mu (3 \eta \mu^2 + \lambda \mu^1 + 3 \mu \rho) + \\
& \quad \delta \mu (3 \eta^2 \mu^3 + 2 \eta \mu (5 \lambda \mu^1 - 3 \mu \rho) + \rho (-2 \lambda \mu^1 + 3 \mu \rho)) + \\
& \quad \lambda \mu^1 (-8 \eta^2 \mu^3 + 4 \eta \mu^2 \rho + \rho (\lambda \mu^1 + 4 \mu \rho)) + \\
& \quad \beta \theta \mu (3 \delta^3 \mu + 3 \eta^3 \mu^4 - \rho^2 (2 \lambda \mu^1 + 3 \mu \rho) - \delta^2 (3 \eta \mu^2 + 2 \lambda \mu^1 + 9 \mu \rho) + \eta \mu \rho (4 \lambda \mu^1 + 9 \mu \rho) - \\
& \quad \eta^2 \mu^2 (8 \lambda \mu^1 + 9 \mu \rho) + \delta (-3 \eta^2 \mu^3 + 2 \eta \mu (5 \lambda \mu^1 - 3 \mu \rho) + \rho (4 \lambda \mu^1 + 9 \mu \rho))) - \\
& \beta^2 \eta (-3 \delta^4 \eta \mu^2 + 4 \delta \lambda \mu^1 (\eta^3 \mu^3 - 3 \eta \mu \rho^2 + 6 \rho^3 + 2 \eta^2 \mu (\lambda \mu^1 - 2 \mu \rho)) + \\
& \quad 2 \delta^3 (3 \eta^2 \mu^3 + 4 \lambda \mu^1 \rho + \eta \mu (8 \lambda \mu^1 + 3 \mu \rho)) + \\
& \quad 4 \lambda \mu^1 (3 \eta^4 \mu^4 - 2 \rho^4 + 3 \eta^2 \mu \rho (\lambda \mu^1 + \mu \rho) + \eta \rho^2 (4 \lambda \mu^1 + 3 \mu \rho) - \eta^3 \mu^2 (\lambda \mu^1 + 7 \mu \rho)) - \\
& \quad \delta^2 (3 \eta^3 \mu^4 + 24 \lambda \mu^1 \rho^2 + 2 \eta^2 \mu^2 (16 \lambda \mu^1 - 3 \mu \rho) + \eta (4 \lambda^2 \mu^1 + 16 \lambda \mu \mu^1 \rho + 3 \mu^2 \rho^2)) - \\
& \quad \beta \theta^2 \mu (3 \delta^3 \mu^2 - 2 \delta^2 \mu (3 \eta \mu^2 + \lambda \mu^1 + 3 \mu \rho) + \\
& \quad \delta \mu (3 \eta^2 \mu^3 + 2 \eta \mu (5 \lambda \mu^1 - 3 \mu \rho) + \rho (-2 \lambda \mu^1 + 3 \mu \rho)) + \lambda \mu^1 \\
& \quad (-8 \eta^2 \mu^3 + 4 \eta \mu^2 \rho + \rho (\lambda \mu^1 + 4 \mu \rho)) + \beta \theta (-3 \delta^4 \mu^2 + \delta^3 \mu (3 \eta \mu^2 + 16 \lambda \mu^1 + 9 \mu \rho) + \\
& \quad \delta^2 (3 \eta^2 \mu^4 - 4 \lambda^2 \mu^1 - 26 \lambda \mu \mu^1 \rho - 9 \mu^2 \rho^2 + 6 \eta \mu^2 (-5 \lambda \mu^1 + \mu \rho)) + \\
& \quad 2 \lambda \mu^1 (10 \eta^3 \mu^4 + 4 \eta \mu \rho (\lambda \mu^1 + \mu \rho) + \rho^2 (2 \lambda \mu^1 + 3 \mu \rho) - \eta^2 \mu^2 (2 \lambda \mu^1 + 17 \mu \rho)) + \\
& \quad \delta \mu (-3 \eta^3 \mu^4 + \rho^2 (4 \lambda \mu^1 + 3 \mu \rho) + \eta^2 (-6 \lambda \mu^2 \mu^1 + 9 \mu^3 \rho) + \eta (8 \lambda^2 \mu^1 - 9 \mu^2 \rho^2))) + \\
& \beta (\beta \theta^2 \mu^2 (3 \delta^3 \mu + 3 \eta^3 \mu^4 - \rho^2 (2 \lambda \mu^1 + 3 \mu \rho) - \delta^2 (3 \eta \mu^2 + 2 \lambda \mu^1 + 9 \mu \rho) + \\
& \quad \eta \mu \rho (4 \lambda \mu^1 + 9 \mu \rho) - \eta^2 \mu^2 (8 \lambda \mu^1 + 9 \mu \rho) + \\
& \quad \delta (-3 \eta^2 \mu^3 + 2 \eta \mu (5 \lambda \mu^1 - 3 \mu \rho) + \rho (4 \lambda \mu^1 + 9 \mu \rho)) + \beta \theta (3 \delta^4 \mu^2 + 3 \eta^4 \mu^6 - \\
& \quad 4 \delta^3 \mu (4 \lambda \mu^1 + 3 \mu \rho) - 4 \eta^3 \mu^4 (7 \lambda \mu^1 + 3 \mu \rho) + \rho^2 (4 \lambda^2 \mu^1 + 16 \lambda \mu \mu^1 \rho + 3 \mu^2 \rho^2) - \\
& \quad 2 \eta \mu \rho (5 \lambda^2 \mu^1 + 12 \lambda \mu \mu^1 \rho + 6 \mu^2 \rho^2) + 2 \eta^2 \mu^2 (2 \lambda^2 \mu^1 + 18 \lambda \mu \mu^1 \rho + 9 \mu^2 \rho^2) + \\
& \quad \delta^2 (-6 \eta^2 \mu^4 + 4 \lambda^2 \mu^1 + 48 \lambda \mu \mu^1 \rho + 18 \mu^2 \rho^2 + 4 \eta \mu^2 (7 \lambda \mu^1 - 3 \mu \rho)) + \\
& \quad 4 \delta (\eta^2 \mu^3 (4 \lambda \mu^1 - 3 \mu \rho) - \rho (2 \lambda^2 \mu^1 + 12 \lambda \mu \mu^1 \rho + 3 \mu^2 \rho^2) + \eta \mu \\
& \quad (-2 \lambda^2 \mu^1 - \lambda \mu \mu^1 \rho + 6 \mu^2 \rho^2))) + \eta (3 \delta^4 \mu^2 - \delta^3 \mu (3 \eta \mu^2 + 16 \lambda \mu^1 + 9 \mu \rho) +
\end{aligned}$$

$$\begin{aligned}
& \delta^2 \left(-3 \eta^2 \mu^4 + 4 \lambda^2 \mu^2 + 26 \lambda \mu \rho + 9 \mu^2 \rho^2 - 6 \eta \mu^2 (-5 \lambda \mu + \mu \rho) \right) + \\
& 2 \lambda \mu \left(-10 \eta^3 \mu^4 - 4 \eta \mu \rho (\lambda \mu + \mu \rho) - \rho^2 (2 \lambda \mu + 3 \mu \rho) + \eta^2 \mu^2 (2 \lambda \mu + 17 \mu \rho) \right) + \\
& \delta \mu \left(3 \eta^3 \mu^4 + 3 \eta^2 \mu^2 (2 \lambda \mu - 3 \mu \rho) - \rho^2 (4 \lambda \mu + 3 \mu \rho) + \eta (-8 \lambda^2 \mu^2 + 9 \mu^2 \rho^2) \right) + \\
\alpha^3 & \left(-\mu \left(2 \beta \theta^2 \mu^2 (\delta^2 - 5 \delta \eta \mu + 4 \eta^2 \mu^2 - 2 \delta \rho - 5 \eta \mu \rho + \rho^2) + \eta (-4 \delta^3 \mu + \delta^2 (2 \eta \mu^2 + \lambda \mu + 8 \mu \rho) + \right. \right. \\
& 2 \delta \mu (\eta^2 \mu^2 + \eta \lambda \mu + \eta \mu \rho - 2 \rho^2) - \lambda \mu (6 \eta^2 \mu^2 + 2 \eta \mu \rho + \rho^2) \left. \right) + \\
& \beta \theta \left(-4 \delta^3 \mu + 8 \eta^3 \mu^4 - 2 \eta \lambda \mu \rho - 6 \eta^2 \mu^2 (\lambda \mu + 2 \mu \rho) + \rho^2 (\lambda \mu + 4 \mu \rho) + \right. \\
& \delta^2 (4 \eta \mu^2 + \lambda \mu + 12 \mu \rho) - 2 \delta (4 \eta^2 \mu^3 + \eta \mu (-\lambda \mu + 2 \mu \rho) + \rho (\lambda \mu + 6 \mu \rho)) \left. \right) + \\
\beta^3 & \eta \left(\beta \theta^3 \mu (4 \delta^3 \mu - \delta^2 (2 \eta \mu^2 + \lambda \mu + 8 \mu \rho) - 2 \delta \mu (\eta^2 \mu^2 + \eta \lambda \mu + \eta \mu \rho - 2 \rho^2) + \right. \\
& \lambda \mu (6 \eta^2 \mu^2 + 2 \eta \mu \rho + \rho^2) \left. \right) + \\
& 4 \eta (2 \delta^5 - 2 \delta^4 (2 \eta \mu + 3 \rho) + 4 \delta \eta \lambda \mu (4 \eta^2 \mu^2 + \eta \lambda \mu - 3 \eta \mu \rho - \rho^2) + \\
& \eta \lambda \mu (\eta \mu - \rho) (3 \eta^2 \mu^2 - 4 \eta \lambda \mu - 6 \eta \mu \rho + 3 \rho^2) + \delta^3 (5 \eta^2 \mu^2 + 3 \eta \mu \rho + 6 \rho^2) + \\
& \delta^2 (-3 \eta^3 \mu^3 - 2 \rho^3 + 4 \eta^2 \mu (-4 \lambda \mu + \mu \rho) + \eta \rho (4 \lambda \mu + \mu \rho)) \left. \right) + \\
\beta \theta^2 & (6 \delta^4 \mu - 2 \delta^3 (\eta \mu^2 + 2 \lambda \mu + 9 \mu \rho) + \eta \lambda \mu (26 \eta^2 \mu^2 - 8 \eta \lambda \mu - 29 \eta \mu \rho + 3 \rho^2) + \\
& \delta^2 (10 \eta^2 \mu^3 + \eta \mu (-25 \lambda \mu + 4 \mu \rho) + 2 \rho (4 \lambda \mu + 9 \mu \rho)) - 2 \delta (7 \eta^3 \mu^4 + \rho^2 \\
& (2 \lambda \mu + 3 \mu \rho) - \eta^2 \mu^2 (9 \lambda \mu + 11 \mu \rho) + \eta (-4 \lambda^2 \mu^2 - 12 \lambda \mu \rho + \mu^2 \rho^2)) \left. \right) + \\
2 \beta \theta & (4 \delta^5 - \delta^4 (5 \eta \mu + 16 \rho) + \delta^3 (7 \eta^2 \mu^2 - 2 \eta \lambda \mu + 4 \eta \mu \rho + 24 \rho^2) + \\
& \delta^2 (-16 \rho^3 + \eta \rho (10 \lambda \mu + 7 \mu \rho) + \eta^2 \mu (-44 \lambda \mu + 9 \mu \rho)) \left. \right) + \\
& 2 \eta \lambda \mu (8 \eta^3 \mu^3 - \rho^3 + 2 \eta \rho (2 \lambda \mu + 5 \mu \rho) - \eta^2 \mu (6 \lambda \mu + 17 \mu \rho)) - 2 \delta (3 \eta^4 \mu^4 - 2 \rho^4 + \\
& 3 \eta \rho^2 (\lambda \mu + \mu \rho) - 7 \eta^3 \mu^2 (3 \lambda \mu + \mu \rho) + \eta^2 (-6 \lambda^2 \mu^2 + 5 \lambda \mu \rho + 3 \mu^2 \rho^2)) \left. \right) + \\
\beta & (-2 \beta \theta^3 \mu^3 (\delta^2 - 5 \delta \eta \mu + 4 \eta^2 \mu^2 - 2 \delta \rho - 5 \eta \mu \rho + \rho^2) + 2 \beta \theta^2 \mu (-4 \delta^3 \mu - 14 \eta^3 \mu^4 + \\
& 3 \delta^2 (4 \eta \mu^2 + \lambda \mu + 4 \mu \rho) + \rho^2 (3 \lambda \mu + 4 \mu \rho) - 2 \eta \mu \rho (3 \lambda \mu + 11 \mu \rho) + \\
& 2 \eta^2 \mu^2 (5 \lambda \mu + 16 \mu \rho) + 2 \delta (3 \eta^2 \mu^3 + 5 \eta \mu (-\lambda \mu + \mu \rho) - 3 \rho (\lambda \mu + 2 \mu \rho)) \left. \right) + \\
\eta & (6 \delta^4 \mu - 2 \delta^3 (\eta \mu^2 + 2 \lambda \mu + 9 \mu \rho) + \eta \lambda \mu (26 \eta^2 \mu^2 - 8 \eta \lambda \mu - 29 \eta \mu \rho + 3 \rho^2) + \\
& \delta^2 (10 \eta^2 \mu^3 + \eta \mu (-25 \lambda \mu + 4 \mu \rho) + 2 \rho (4 \lambda \mu + 9 \mu \rho)) - 2 \delta (7 \eta^3 \mu^4 + \rho^2 \\
& (2 \lambda \mu + 3 \mu \rho) - \eta^2 \mu^2 (9 \lambda \mu + 11 \mu \rho) + \eta (-4 \lambda^2 \mu^2 - 12 \lambda \mu \rho + \mu^2 \rho^2)) \left. \right) + \\
\beta \theta & (6 \delta^4 \mu - 20 \eta^4 \mu^5 + \eta \mu \rho^2 (3 \lambda \mu + 2 \mu \rho) + 2 \rho^3 (2 \lambda \mu + 3 \mu \rho) - 2 \delta^3 (5 \eta \mu^2 + \\
& 2 \lambda \mu + 12 \mu \rho) + 2 \eta^3 \mu^3 (23 \lambda \mu + 27 \mu \rho) - 2 \eta^2 \mu (4 \lambda^2 \mu^2 + 23 \lambda \mu \rho + 21 \mu^2 \rho^2) + \\
& \delta^2 (36 \eta^2 \mu^3 + 12 \rho (\lambda \mu + 3 \mu \rho) + \eta \mu (-19 \lambda \mu + 22 \mu \rho)) - 2 \delta (6 \eta^3 \mu^4 + \eta^2 \\
& \mu^2 (\lambda \mu - 25 \mu \rho) + 6 \rho^2 (\lambda \mu + 2 \mu \rho) + \eta (-4 \lambda^2 \mu^2 - 8 \lambda \mu \rho + 7 \mu^2 \rho^2)) \left. \right) + \\
\beta^2 & (\beta \theta^3 \mu (4 \delta^3 \mu - 8 \eta^3 \mu^4 + 2 \eta \lambda \mu \rho + 6 \eta^2 \mu^2 (\lambda \mu + 2 \mu \rho) - \rho^2 (\lambda \mu + 4 \mu \rho) - \\
& \delta^2 (4 \eta \mu^2 + \lambda \mu + 12 \mu \rho) + 2 \delta (4 \eta^2 \mu^3 + \eta \mu (-\lambda \mu + 2 \mu \rho) + \rho (\lambda \mu + 6 \mu \rho)) \left. \right) + \\
& 2 \eta (4 \delta^5 - \delta^4 (5 \eta \mu + 16 \rho) + \delta^3 (7 \eta^2 \mu^2 - 2 \eta \lambda \mu + 4 \eta \mu \rho + 24 \rho^2) + \\
& \delta^2 (-16 \rho^3 + \eta \rho (10 \lambda \mu + 7 \mu \rho) + \eta^2 \mu (-44 \lambda \mu + 9 \mu \rho)) \left. \right) + \\
& 2 \eta \lambda \mu (8 \eta^3 \mu^3 - \rho^3 + 2 \eta \rho (2 \lambda \mu + 5 \mu \rho) - \eta^2 \mu (6 \lambda \mu + 17 \mu \rho)) - 2 \delta (3 \eta^4 \mu^4 - 2 \rho^4 + \\
& 3 \eta \rho^2 (\lambda \mu + \mu \rho) - 7 \eta^3 \mu^2 (3 \lambda \mu + \mu \rho) + \eta^2 (-6 \lambda^2 \mu^2 + 5 \lambda \mu \rho + 3 \mu^2 \rho^2)) \left. \right) + \\
\beta \theta^2 & (6 \delta^4 \mu - 20 \eta^4 \mu^5 + \eta \mu \rho^2 (3 \lambda \mu + 2 \mu \rho) + 2 \rho^3 (2 \lambda \mu + 3 \mu \rho) - 2 \delta^3 (5 \eta \mu^2 + \\
& 2 \lambda \mu + 12 \mu \rho) + 2 \eta^3 \mu^3 (23 \lambda \mu + 27 \mu \rho) - 2 \eta^2 \mu (4 \lambda^2 \mu^2 + 23 \lambda \mu \rho + 21 \mu^2 \rho^2) + \\
& \delta^2 (36 \eta^2 \mu^3 + 12 \rho (\lambda \mu + 3 \mu \rho) + \eta \mu (-19 \lambda \mu + 22 \mu \rho)) - 2 \delta (6 \eta^3 \mu^4 + \eta^2 \\
& \mu^2 (\lambda \mu - 25 \mu \rho) + 6 \rho^2 (\lambda \mu + 2 \mu \rho) + \eta (-4 \lambda^2 \mu^2 - 8 \lambda \mu \rho + 7 \mu^2 \rho^2)) \left. \right) + \\
2 \beta \theta & (4 \delta^5 - 6 \eta^5 \mu^5 - 4 \rho^5 - 2 \delta^4 (\eta \mu + 10 \rho) + 2 \eta \rho^3 (4 \lambda \mu + 5 \mu \rho) + \\
& 4 \eta^4 \mu^3 (9 \lambda \mu + 5 \mu \rho) + \eta^2 \lambda \mu \rho (8 \lambda \mu + 17 \mu \rho) -
\end{aligned}$$

$$\begin{aligned}
& 4 \delta^3 (\eta \lambda \mu 1 + \eta \mu \rho - 10 \rho^2) - \eta^3 \mu (16 \lambda^2 \mu 1^2 + 61 \lambda \mu \mu 1 \rho + 20 \mu^2 \rho^2) + \\
& \delta^2 (20 \eta^3 \mu^3 - 40 \rho^3 + 8 \eta \rho (2 \lambda \mu 1 + 3 \mu \rho) + \eta^2 \mu (-53 \lambda \mu 1 + 20 \mu \rho)) - 2 \delta (8 \eta^4 \mu^4 - 10 \\
& \rho^4 + 2 \eta \rho^2 (5 \lambda \mu 1 + 7 \mu \rho) - \eta^3 \mu^2 (21 \lambda \mu 1 + 22 \mu \rho) + \eta^2 (-8 \lambda^2 \mu 1^2 + 10 \mu^2 \rho^2)) + \\
& \alpha^4 (\mu (\delta \eta (\delta^2 + 6 \delta \eta \mu - 4 \eta^2 \mu^2 - 2 \eta \lambda \mu 1 - 2 \delta \rho - 6 \eta \mu \rho + \rho^2) - \beta \theta^2 \mu \\
& (\delta^2 + 2 \delta \eta \mu - 6 \eta^2 \mu^2 - 2 \delta \rho + 5 \eta \mu \rho + \rho^2) + \beta \theta (\delta^3 + 6 \eta^3 \mu^3 + \delta^2 (5 \eta \mu - 3 \rho) - \\
& 4 \eta^2 \mu^2 \rho - \eta \mu \rho^2 - \rho^3 - \delta (6 \eta^2 \mu^2 + 2 \eta \lambda \mu 1 + 4 \eta \mu \rho - 3 \rho^2))) + \\
& \beta^4 \eta (\beta \theta^4 \delta \mu (\delta^2 + 6 \delta \eta \mu - 4 \eta^2 \mu^2 - 2 \eta \lambda \mu 1 - 2 \delta \rho - 6 \eta \mu \rho + \rho^2) + \\
& 4 \eta^3 (8 \delta^4 + 4 \eta^2 \lambda^2 \mu 1^2 - 16 \delta \eta \lambda \mu 1 (\eta \mu - \rho) + 3 \delta^2 (-\eta \mu + \rho)^2 - 4 \delta^3 (2 \eta \mu + 3 \rho)) + \\
& \beta \theta^2 \eta (16 \delta^4 + 4 \delta^3 (5 \eta \mu - 13 \rho) - \delta^2 (5 \eta^2 \mu^2 + 24 \eta \lambda \mu 1 + 67 \eta \mu \rho - 56 \rho^2) + \\
& 4 \eta \lambda \mu 1 (-3 \eta^2 \mu^2 - 2 \rho^2 + 5 \eta (\lambda \mu 1 + \mu \rho)) + \\
& 4 \delta (2 \eta^3 \mu^3 - 5 \rho^3 + 12 \eta \rho (\lambda \mu 1 + \mu \rho) - 3 \eta^2 \mu (5 \lambda \mu 1 + 3 \mu \rho))) + \\
& 4 \beta \theta \eta^2 (12 \delta^4 - \delta^3 (6 \eta \mu + 25 \rho) - 4 \delta^2 (\eta \lambda \mu 1 + 4 \eta \mu \rho - 4 \rho^2) - 2 \eta \lambda \mu 1 (\eta^2 \mu^2 + \rho^2 - \\
& 2 \eta (2 \lambda \mu 1 + \mu \rho)) + \delta (3 \eta^3 \mu^3 - 3 \rho^3 + \eta \rho (26 \lambda \mu 1 + 9 \mu \rho) - \eta^2 \mu (28 \lambda \mu 1 + 9 \mu \rho))) + \\
& \beta \theta^3 \eta (13 \delta^3 \mu + \delta^2 (13 \eta \mu^2 - 8 \lambda \mu 1 - 28 \mu \rho) + 4 \eta \lambda \mu 1 (-\eta \mu^2 + \lambda \mu 1 + \mu \rho) + \\
& \delta (-8 \eta^2 \mu^3 - 7 \eta \mu (2 \lambda \mu 1 + \mu \rho) + \rho (8 \lambda \mu 1 + 15 \mu \rho))) + \\
& \beta (2 \beta \theta^3 \mu^2 (\delta^2 + 8 \eta^2 \mu^2 - 9 \eta \mu \rho + \rho^2 - 2 \delta (3 \eta \mu + \rho)) + \beta \theta^2 \mu \\
& (-\delta^3 + 42 \eta^3 \mu^3 + \rho^3 + \delta^2 (-5 \eta \mu + 3 \rho) - 4 \eta^2 \mu (4 \lambda \mu 1 + 19 \mu \rho) + \\
& \eta \rho (8 \lambda \mu 1 + 33 \mu \rho) - \delta (6 \eta^2 \mu^2 - 10 \eta \lambda \mu 1 + 28 \eta \mu \rho + 3 \rho^2))) + \\
& \beta \theta \eta (12 \delta^3 \mu + 26 \eta^3 \mu^4 - 3 \mu \rho^3 + \delta^2 (6 \eta \mu^2 - 8 \lambda \mu 1 - 27 \mu \rho) - 5 \eta^2 \mu^2 (4 \lambda \mu 1 + 11 \mu \rho) + \\
& 4 \eta (\lambda^2 \mu 1^2 + 3 \lambda \mu \mu 1 \rho + 8 \mu^2 \rho^2) - 2 \delta (\eta^2 \mu^3 + 2 \eta \mu (\lambda \mu 1 + 8 \mu \rho) - \rho (4 \lambda \mu 1 + 9 \mu \rho))) + \\
& \eta^2 (13 \delta^3 \mu + \delta^2 (13 \eta \mu^2 - 8 \lambda \mu 1 - 28 \mu \rho) + 4 \eta \lambda \mu 1 (-\eta \mu^2 + \lambda \mu 1 + \mu \rho) + \\
& \delta (-8 \eta^2 \mu^3 - 7 \eta \mu (2 \lambda \mu 1 + \mu \rho) + \rho (8 \lambda \mu 1 + 15 \mu \rho))) - \\
& \beta^2 (\beta \theta^4 \mu^2 (\delta^2 + 2 \delta \eta \mu - 6 \eta^2 \mu^2 - 2 \delta \rho + 5 \eta \mu \rho + \rho^2) + \beta \theta^3 \mu (\delta^3 - 42 \eta^3 \mu^3 + \delta^2 (5 \eta \mu - 3 \rho) - \rho^3 + \\
& 4 \eta^2 \mu (4 \lambda \mu 1 + 19 \mu \rho) - \eta \rho (8 \lambda \mu 1 + 33 \mu \rho) + \delta (6 \eta^2 \mu^2 - 10 \eta \lambda \mu 1 + 28 \eta \mu \rho + 3 \rho^2))) + \\
& \eta^2 (-16 \delta^4 + \delta^3 (-20 \eta \mu + 52 \rho) + \delta^2 (5 \eta^2 \mu^2 + 24 \eta \lambda \mu 1 + 67 \eta \mu \rho - 56 \rho^2) + \\
& 4 \eta \lambda \mu 1 (3 \eta^2 \mu^2 + 2 \rho^2 - 5 \eta (\lambda \mu 1 + \mu \rho)) - \\
& 4 \delta (2 \eta^3 \mu^3 - 5 \rho^3 + 12 \eta \rho (\lambda \mu 1 + \mu \rho) - 3 \eta^2 \mu (5 \lambda \mu 1 + 3 \mu \rho))) - \\
& 2 \beta \theta^2 \eta (11 \delta^3 \mu + 34 \eta^3 \mu^4 - \rho^2 (8 \lambda \mu 1 + 19 \mu \rho) - 3 \eta^2 \mu^2 (12 \lambda \mu 1 + 29 \mu \rho) - \\
& \delta^2 (30 \eta \mu^2 + 8 \lambda \mu 1 + 41 \mu \rho) + 4 \eta (\lambda^2 \mu 1^2 + 9 \lambda \mu \mu 1 \rho + 18 \mu^2 \rho^2) + \\
& \delta (30 \eta^2 \mu^3 + 2 \eta \mu (7 \lambda \mu 1 - 47 \mu \rho) + \rho (16 \lambda \mu 1 + 49 \mu \rho))) + \\
& \beta \theta \eta (-16 \delta^4 + \delta^3 (-43 \eta \mu + 52 \rho) + \delta^2 (61 \eta^2 \mu^2 - 60 \rho^2 + 8 \eta (5 \lambda \mu 1 + 19 \mu \rho)) + \\
& \delta (-72 \eta^3 \mu^3 + 28 \rho^3 - \eta \rho (80 \lambda \mu 1 + 153 \mu \rho) + \eta^2 \mu (42 \lambda \mu 1 + 197 \mu \rho)) - \\
& 4 (8 \eta^4 \mu^4 + \rho^4 - \eta \rho^2 (6 \lambda \mu 1 + 11 \mu \rho) - \eta^3 \mu^2 \\
& (17 \lambda \mu 1 + 25 \mu \rho) + \eta^2 (7 \lambda^2 \mu 1^2 + 21 \lambda \mu \mu 1 \rho + 27 \mu^2 \rho^2))) + \\
& \beta^3 (\beta \theta^4 \mu (\delta^3 + 6 \eta^3 \mu^3 + \delta^2 (5 \eta \mu - 3 \rho) - 4 \eta^2 \mu^2 \rho - \eta \mu \rho^2 - \rho^3 - \\
& \delta (6 \eta^2 \mu^2 + 2 \eta \lambda \mu 1 + 4 \eta \mu \rho - 3 \rho^2)) + \\
& \beta \theta^3 \eta (12 \delta^3 \mu + 26 \eta^3 \mu^4 - 3 \mu \rho^3 + \delta^2 (6 \eta \mu^2 - 8 \lambda \mu 1 - 27 \mu \rho) - 5 \eta^2 \mu^2 (4 \lambda \mu 1 + 11 \mu \rho) + \\
& 4 \eta (\lambda^2 \mu 1^2 + 3 \lambda \mu \mu 1 \rho + 8 \mu^2 \rho^2) - 2 \delta (\eta^2 \mu^3 + 2 \eta \mu (\lambda \mu 1 + 8 \mu \rho) - \rho (4 \lambda \mu 1 + 9 \mu \rho))) + \\
& 4 \eta^3 (12 \delta^4 - \delta^3 (6 \eta \mu + 25 \rho) - 4 \delta^2 (\eta \lambda \mu 1 + 4 \eta \mu \rho - 4 \rho^2) - \\
& 2 \eta \lambda \mu 1 (\eta^2 \mu^2 + \rho^2 - 2 \eta (2 \lambda \mu 1 + \mu \rho)) + \\
& \delta (3 \eta^3 \mu^3 - 3 \rho^3 + \eta \rho (26 \lambda \mu 1 + 9 \mu \rho) - \eta^2 \mu (28 \lambda \mu 1 + 9 \mu \rho))) + 2 \beta \theta \eta^2
\end{aligned}$$

$$\begin{aligned}
& (32 \delta^4 + 6 \eta^4 \mu^4 + 4 \delta^3 (\eta \mu - 19 \rho) + 6 \rho^4 - 8 \eta \rho^2 (2 \lambda \mu 1 + 3 \mu \rho) - 4 \eta^3 \mu^2 (7 \lambda \mu 1 + 6 \mu \rho) - \\
& \delta^2 (31 \eta^2 \mu^2 + 24 \eta \lambda \mu 1 + 95 \eta \mu \rho - 62 \rho^2) + 4 \eta^2 (7 \lambda^2 \mu 1^2 + 11 \lambda \mu \mu 1 \rho + 9 \mu^2 \rho^2) + \\
& 4 \delta (10 \eta^3 \mu^3 - 6 \rho^3 + 22 \eta \rho (\lambda \mu 1 + \mu \rho) - \eta^2 \mu (19 \lambda \mu 1 + 26 \mu \rho)) + \\
& \beta 0^2 \eta (16 \delta^4 + \delta^3 (43 \eta \mu - 52 \rho) - \delta^2 (61 \eta^2 \mu^2 - 60 \rho^2 + 8 \eta (5 \lambda \mu 1 + 19 \mu \rho)) + \\
& \delta (72 \eta^3 \mu^3 - 28 \rho^3 + \eta \rho (80 \lambda \mu 1 + 153 \mu \rho) - \eta^2 \mu (42 \lambda \mu 1 + 197 \mu \rho)) + \\
& 4 (8 \eta^4 \mu^4 + \rho^4 - \eta \rho^2 (6 \lambda \mu 1 + 11 \mu \rho) - \eta^3 \mu^2 \\
& (17 \lambda \mu 1 + 25 \mu \rho) + \eta^2 (7 \lambda^2 \mu 1^2 + 21 \lambda \mu \mu 1 \rho + 27 \mu^2 \rho^2)))));
\end{aligned}$$